Test/Interpreter/Arith/remsi.mlir
@@ -3,15 +3,13 @@
 "builtin.module"() ({
   %lhs = "arith.constant"() <{ "value" = 7 : i32 }> : () -> i32
   %rhs = "arith.constant"() <{ "value" = 2 : i32 }> : () -> i32
-  %zero = "arith.constant"() <{ "value" = 0 : i32 }> : () -> i32
   %negone = "arith.constant"() <{ "value" = -1 : i32 }> : () -> i32
   %negthree = "arith.constant"() <{ "value" = -3 : i32 }> : () -> i32
   %negtwo = "arith.constant"() <{ "value" = -2 : i32 }> : () -> i32
   %x = "arith.remsi"(%lhs, %rhs) : (i32, i32) -> i32
-  %y = "arith.remsi"(%lhs, %zero) : (i32, i32) -> i32
   %z = "arith.remsi"(%lhs, %negone) : (i32, i32) -> i32
   %a = "arith.remsi"(%negthree, %negtwo) : (i32, i32) -> i32
-  "func.return"(%x, %y, %z, %a) : (i32, i32, i32, i32) -> ()
+  "func.return"(%x, %z, %a) : (i32, i32, i32) -> ()
 }) : () -> ()
 
-// CHECK: Program output: #[0x00000001#32, poison, 0x00000000#32, 0xffffffff#32]
+// CHECK: Program output: #[0x00000001#32, 0x00000000#32, 0xffffffff#32]
