Test/Interpreter/LLVM/urem.mlir
@@ -3,13 +3,11 @@
 "builtin.module"() ({
   %lhs = "llvm.mlir.constant"() <{ "value" = 130 : i32 }> : () -> i32
   %rhs = "llvm.mlir.constant"() <{ "value" = 3 : i32 }> : () -> i32
-  %zero = "llvm.mlir.constant"() <{ "value" = 0 : i32 }> : () -> i32
   %negthree = "llvm.mlir.constant"() <{ "value" = -3 : i32 }> : () -> i32
   %negtwo = "llvm.mlir.constant"() <{ "value" = -2 : i32 }> : () -> i32
   %x = "llvm.urem"(%lhs, %rhs) : (i32, i32) -> i32
-  %y = "llvm.urem"(%lhs, %zero) : (i32, i32) -> i32
   %a = "llvm.urem"(%negthree, %negtwo) : (i32, i32) -> i32
-  "func.return"(%x, %y, %a) : (i32, i32, i32) -> ()
+  "func.return"(%x, %a) : (i32, i32) -> ()
 }) : () -> ()
 
-// CHECK: Program output: #[0x00000001#32, poison, 0xfffffffd#32]
+// CHECK: Program output: #[0x00000001#32, 0xfffffffd#32]
